Eliminate dead code (#53); fix 3 unreplayable hints (including the top worst offender)

code/bignum/Hacl.Bignum.Fmul.fst
@@ -51,49 +51,61 @@ val mul_shift_reduce_:
       /\ (let output', input' = mul_shift_reduce_spec_ (as_seq h0 output) (as_seq h0 input) (as_seq h0 input) (as_seq h0 input2) (0) in
          as_seq h1 output == output')
       ))
-#reset-options "--z3rlimit 1000 --initial_fuel 1 --max_fuel 1"
+#reset-options "--z3rlimit 200 --initial_fuel 1 --max_fuel 1"
+
 let mul_shift_reduce_ output input input2 =
   let h0 = ST.get() in
-  let inv (h1: HyperStack.mem) (i: nat): Type0 =
-    live h1 output /\ live h1 input /\ modifies_2 output input h0 h1 /\ 0 <= i /\ i <= len /\
-    (let output', input' = mul_shift_reduce_spec_ (as_seq h0 output) (as_seq h0 input) (as_seq h0 input) (as_seq h0 input2) (len - i) in
-     as_seq h1 output == output' /\ as_seq h1 input == input')
+  let inv h i =
+    live h output /\ live h input /\ modifies_2 output input h0 h /\ 0 <= i /\ i < len /\
+    (let output', input' =
+      mul_shift_reduce_spec_
+        (as_seq h0 output) (as_seq h0 input)
+        (as_seq h0 input) (as_seq h0 input2)
+        (len - i) in
+     as_seq h output == output' /\ as_seq h input == input')
   in
-  let f' (i:UInt32.t{FStar.UInt32.( 0 <= v i /\ v i < len) }): Stack unit
-    (requires (fun h -> inv h (UInt32.v i)))
-    (ensures (fun h_1 _ h_2 -> FStar.UInt32.(inv h_2 (v i + 1))))
+  let f' (i:U32.t{0 <= U32.v i /\ U32.v i < len - 1}) : Stack unit
+    (requires (fun h -> inv h (U32.v i)))
+    (ensures  (fun _ _ h1 -> inv h1 (U32.v i + 1)))
   = let h0' = ST.get() in
-    lemma_mul_shift_reduce_spec_def (as_seq h0 output) (as_seq h0 input) (as_seq h0 input) (as_seq h0 input2) (len - UInt32.v i - 1);
-    let ctr = FStar.UInt32.(clen -^ i -^ 1ul) in
-    let i = FStar.UInt32.(ctr) in
-    let j = FStar.UInt32.(clen -^ 1ul -^ i) in
-    let input2i = input2.(j) in
-    Hacl.Spec.Bignum.Fproduct.lemma_sum_scalar_multiplication_ (as_seq h0' output) (as_seq h0' input)
-                                                               (input2i) len;
+    lemma_mul_shift_reduce_spec_def
+      (as_seq h0 output) (as_seq h0 input)
+      (as_seq h0 input) (as_seq h0 input2)
+      (len - U32.v i - 1);
+    let input2i = input2.(i) in
+    Hacl.Spec.Bignum.Fproduct.lemma_sum_scalar_multiplication_
+      (as_seq h0' output) (as_seq h0' input) (input2i) len;
     sum_scalar_multiplication_ output input input2i;
-    if FStar.UInt32.(ctr >^ 0ul) then shift_reduce input;
+    let h1 = ST.get() in
+    shift_reduce input;
     let h' = ST.get() in
-    if FStar.UInt32.(ctr >^ 0ul) then (
-      let open Hacl.Bignum.Limb in
-      lemma_shift_reduce_spec (as_seq h0' input);
-      lemma_mul_shift_reduce_spec_1 (as_seq h' output) (as_seq h0' output) (as_seq h0 input)
-                                   (as_seq h0' input) (as_seq h' input) (as_seq h0' input2)
-                                   (v input2i) (FStar.UInt32.v ctr + 1);
-      ()
-    ) else (
-      let open Hacl.Bignum.Limb in
-      lemma_mul_shift_reduce_spec_2 (as_seq h' output) (as_seq h0' output) (as_seq h0 input)
-                                   (as_seq h0' input) (as_seq h' input) (as_seq h0' input2)
-                                   (v input2i);
-      ()
-    )
+    lemma_modifies_1_1 output input h0' h1 h';
+    lemma_modifies_2_trans output input h0 h0' h';
+    lemma_shift_reduce_spec (as_seq h0' input);
+    lemma_mul_shift_reduce_spec_1 (as_seq h' output) (as_seq h0' output) (as_seq h0 input)
+                                  (as_seq h0' input) (as_seq h' input) (as_seq h0' input2)
+                                  (v input2i) (len - U32.v i)
     in
-  lemma_mul_shift_reduce_spec_def_0 (as_seq h0 output) (as_seq h0 input) (as_seq h0 input) (as_seq h0 input2);
-  C.Loops.for 0ul clen inv f'
+  lemma_mul_shift_reduce_spec_def_0
+    (as_seq h0 output) (as_seq h0 input) (as_seq h0 input) (as_seq h0 input2);
+  C.Loops.for 0ul U32.(clen -^ 1ul) inv f';
+  let i = U32.(clen -^ 1ul) in
+  let h0' = ST.get() in
+  lemma_mul_shift_reduce_spec_def
+    (as_seq h0 output) (as_seq h0 input)
+    (as_seq h0 input) (as_seq h0 input2)
+    0;
+  let input2i = input2.(i) in
+  Hacl.Spec.Bignum.Fproduct.lemma_sum_scalar_multiplication_
+    (as_seq h0' output) (as_seq h0' input) (input2i) len;
+  sum_scalar_multiplication_ output input input2i;
+  let h' = ST.get() in
+  lemma_mul_shift_reduce_spec_2 (as_seq h' output) (as_seq h0' output) (as_seq h0 input)
+                                (as_seq h0' input) (as_seq h' input) (as_seq h0' input2)
+                                (v input2i)
 
 
 #reset-options "--z3rlimit 10 --initial_fuel 0 --max_fuel 0"
-
 
 let as_seq' (h:mem) (b:felem{live h b}) : GTot seqelem = as_seq h b
   
@@ -132,8 +144,15 @@ private let fmul_ output input input2 =
   Hacl.Spec.Bignum.Fproduct.lemma_copy_from_wide (as_seq h4 t);
   copy_from_wide_ output t;
   carry_0_to_1 output;
-  let h3 = ST.get() in
-  pop_frame()
+  let h5 = ST.get() in
+  pop_frame();
+  let h6 = ST.get() in
+  lemma_modifies_1_trans t h2' h3 h4;
+  lemma_modifies_0_2 input t h1 h2 h2';
+  lemma_modifies_1_1 t output h2' h4 h5;
+  lemma_modifies_2_1'  t input h2 h2' h4;
+  lemma_modifies_2_1'' input output h1 h4 h5;
+  modifies_popped_3_2 input output h0 h1 h5 h6
 
 
 #reset-options "--z3rlimit 100 --initial_fuel 0 --max_fuel 0"
@@ -157,10 +176,19 @@ let fmul output input input2 =
   push_frame();
   let h1 = ST.get() in
   let tmp = create limb_zero clen in
+  let h1' = ST.get() in
   blit input 0ul tmp 0ul clen;
   let h2 = ST.get() in
   lemma_whole_slice (as_seq h2 input);
   lemma_whole_slice (as_seq h2 tmp);
+  no_upd_lemma_1 h1' h2 tmp output;
+  no_upd_lemma_1 h1' h2 tmp input2;
   fmul_ output tmp input2;
   let h3 = ST.get() in
-  pop_frame()
+  pop_frame();
+  let h4 = ST.get() in
+  lemma_modifies_0_1' tmp h1 h1' h2;
+  lemma_modifies_2_comm tmp output h2 h3;
+  lemma_modifies_1_2'' tmp output h1' h2 h3;
+  lemma_modifies_0_2' output tmp h1 h1' h3;
+  modifies_popped_1 output h0 h1 h3 h4
